gset.fst
@@ -45,7 +45,8 @@ let rec mem_ele ele l =
   |(_, (Add ele1))::xs -> ele = ele1 || mem_ele ele xs
   |(_, Rd)::xs -> mem_ele ele xs
 
-let pre_cond_op s1 op = true
+let pre_cond_app_op s1 op = true
+let pre_cond_prop_oper tr s1 op = true
 
 val app_op : s1:s
            -> op:(nat * op)
@@ -106,45 +107,29 @@ let rec lemma7 tr s1 tr1 =
           else lemma7 (remove_op tr (id, (Add v))) (remove_st v s1) (remove_op tr (id, (Add v)))
              |[], (_, (Add v))::xs -> ()*) ()
 
-val pre_cond_merge1 : l:s -> a:s -> b:s
+val pre_cond_merge : l:s -> a:s -> b:s
                     -> Tot (b1:bool {b1=true <==> (forall e. mem e l ==> mem e a /\ mem e b)})
-let pre_cond_merge1 l a b = 
+let pre_cond_merge l a b = 
   forallb (fun e -> mem e a && mem e b) l
 
-val merge1 : l:s
+val merge : l:s
            -> a:s
            -> b:s
            -> Pure s
-             (requires pre_cond_merge1 l a b)
+             (requires pre_cond_merge l a b)
              (ensures (fun u -> (forall e. mem e u <==> mem e a \/ mem e b)))
              (decreases %[l;a;b])
 
 #set-options "--z3rlimit 10000000"
-let rec merge1 l a b =
+let rec merge l a b =
   match l, a, b with
   |[],[],[] -> []
-  |x::xs, _, _ -> (merge1 xs a b) 
-  |[],x::xs,_ -> if mem x b then (merge1 [] xs b) else x::(merge1 [] xs b)
+  |x::xs, _, _ -> (merge xs a b) 
+  |[],x::xs,_ -> if mem x b then (merge [] xs b) else x::(merge [] xs b)
   |[],[], _ -> b
 
-val pre_cond_merge : ltr:ae op -> l:s -> atr:ae op -> a:s -> btr:ae op -> b:s -> Tot bool
-let pre_cond_merge ltr l atr a btr b = true
-
-val merge : ltr:ae op
-          -> l:s
-          -> atr:ae op
-          -> a:s
-          -> btr:ae op
-          -> b:s
-          -> Pure s (requires (forall e. mem e ltr.l ==> not (mem_id (get_id e) atr.l)) /\
-                             (forall e. mem e atr.l ==> not (mem_id (get_id e) btr.l)) /\
-                             (forall e. mem e ltr.l ==> not (mem_id (get_id e) btr.l)) /\
-                             (sim ltr l /\ sim (union ltr atr) a /\ sim (union ltr btr) b))
-                   (ensures (fun r -> r = merge1 l a b))
-
-#set-options "--z3rlimit 10000000"
-let merge ltr l atr a btr b = 
-  merge1 l a b
+val pre_cond_prop_merge : ltr:ae op -> l:s -> atr:ae op -> a:s -> btr:ae op -> b:s -> Tot bool
+let pre_cond_prop_merge ltr l atr a btr b = true
 
 val prop_merge : ltr:ae op
                -> l:s
@@ -156,7 +141,7 @@ val prop_merge : ltr:ae op
                                  (forall e. mem e atr.l ==> not (mem_id (get_id e) btr.l)) /\
                                  (forall e. mem e ltr.l ==> not (mem_id (get_id e) btr.l)) /\
                                  (sim ltr l /\ sim (union ltr atr) a /\ sim (union ltr btr) b))
-                       (ensures (sim (absmerge ltr atr btr) (merge ltr l atr a btr b)))
+                       (ensures (sim (absmerge ltr atr btr) (merge l a b)))
 
 #set-options "--z3rlimit 10000000"
 let prop_merge ltr l atr a btr b = ()
@@ -193,13 +178,13 @@ instance gset : mrdt s op rval = {
   Library.init = init;
   Library.spec = spec;
   Library.sim = sim;
-  Library.pre_cond_op = pre_cond_op;
-  Library.app_op = app_op;
-  Library.prop_oper = prop_oper;
+  Library.pre_cond_app_op = pre_cond_app_op;
+  Library.pre_cond_prop_oper = pre_cond_prop_oper;
   Library.pre_cond_merge = pre_cond_merge;
-  Library.pre_cond_merge1 = pre_cond_merge1;
-  Library.merge1 = merge1;
+  Library.pre_cond_prop_merge = pre_cond_prop_merge;
+  Library.app_op = app_op;
   Library.merge = merge;
+  Library.prop_oper = prop_oper;
   Library.prop_merge = prop_merge;
   Library.prop_spec = prop_spec;
   Library.convergence = convergence
